theories/L4_deBruijn/classes.v
@@ -1,0 +1,114 @@
+Require Import L4.expression.
+Require Import certiClasses.
+Require Import Common.Common.
+Require Import L3.compile.
+Require Import L4.L3_to_L4.
+Require Import L3.classes.
+
+
+Program Instance : BigStepOpSem L4.expression.exp := eval.
+
+(** FIX!! *)
+Program Instance : WellFormed L4.expression.exp :=
+  fun _  => True.
+
+Instance certiL4: CerticoqLanguage L4.expression.exp := {}.
+
+Program Instance : 
+  CerticoqTranslation (Program L3.compile.Term) L4.expression.exp  :=
+fun p => Ret (L3_to_L4.translate_program (AstCommon.env p) (main p)).
+
+Instance failed: 
+  CerticoqTranslationCorrect (Program L3.compile.Term) L4.expression.exp.
+constructor.
+  compute. auto. 
+
+  intros ? ? Hwf He.
+  destruct Hwf.
+  unfold certiClasses.translate,
+    CerticoqTranslation_instance_0, liftBigStepException, bigStepEval, BigStepOpSem_instance_0.
+  unfold translate_program.
+  Fail eapply L3_to_L4_correct.translate_correct. 
+(* not applicable!! do we need to change the end to end correctness property?, 
+  or can the L3_to_L4 translation syntactically preserve big step eval? *)
+Abort.
+
+Require Import L4_to_L4a.
+Require Import L4a_to_L5.
+Require Import SquiggleEq.export.
+Require Import SquiggleEq.UsefulTypes.
+
+Definition L4aTerm :Type := (@NTerm cps.var CoqL4GenericTermSig).
+
+Program Instance : BigStepOpSem L4aTerm := eval.
+
+(** all variables must be user variables *)
+Program Instance : WellFormed L4aTerm :=
+  fun e  => varsOfClass (all_vars e) true /\ isprogram e.
+
+Instance certiL4a: CerticoqLanguage L4aTerm := {}.
+
+
+Program Instance : 
+  CerticoqTranslation L4.expression.exp L4aTerm :=
+  fun x => Ret (L4_to_L4a x).
+
+
+Definition L5Term :Type := (@NTerm cps.var CPSGenericTermSig).
+
+Program Instance : BigStepOpSem L5Term := eval_c.
+
+Program Instance : WellFormed L5Term := isprogram.
+
+Instance certiL5: CerticoqLanguage L5Term := {}.
+
+Program Instance : 
+  CerticoqTranslation L4aTerm L5Term:=
+  fun x => Ret (cps_cvt x).
+
+
+Require Import L4.L5a.
+
+(* Fix. Define subst and evaluation on L5a by going to L5 via a bijection? *)
+Program Instance : BigStepOpSem L4.L5a.val_c := fun _ _ => True.
+
+(** Fix *)
+Program Instance : WellFormed L4.L5a.val_c := fun x => False.
+
+Instance certiL5a: CerticoqLanguage L5Term := {}.
+
+Program Instance : 
+  CerticoqTranslation  L5Term L4.L5a.val_c :=
+  fun e =>
+   match L4.L5a.translateVal e with
+  | None => exceptionMonad.Exc "error in L5a.translateVal"
+  | Some e => exceptionMonad.Ret e
+  end.
+
+
+Quote Recursively Definition p0L1 := 0.
+
+Require Import L2.classes.
+
+Open Scope Z_scope.
+Require Import ZArith.
+Print Instances CerticoqLanguage.
+Eval compute in (translateTo L5a.val_c p0L1).
+(*
+     = Ret
+         (Cont_c 5%positive
+            (Ret_c (KVar_c 5%positive) (Con_c (mkInd "Coq.Init.Datatypes.nat" 0, 0%N) nil)))
+     : exception val_c
+*)
+
+
+  
+
+
+
+
+
+
+
+
+
