theories/L6_PCPS/L5_to_L6.v
@@ -21,7 +21,7 @@ Require Import CpdtTactics.
 
 
 Require Import ExtLib.Data.List.
-Require Import L4.simpleCPSAA.
+Require Import L4.L4a_to_L5.
 Require Import SquiggleEq.varImplZ.
 Require Import L4.L5a.
 
